ltac experiments

src/Fs7.v
@@ -13,6 +13,8 @@ Definition st_read (s:storage) a :=
 
 Definition empty_storage : storage := fun a => 0.
 
+Print le_S.
+
 Inductive steppable (A:Type) :=
   | step : (storage -> storage * A) -> steppable A
   | mbind : forall B:Type, steppable B -> (B -> steppable A) -> steppable A
@@ -45,7 +47,7 @@ Ltac find_match n :=
   end.
 
 Ltac case_nat n :=
-  try (find_match n; destruct n as [|n]; case_nat n).
+  try (find_match n; destruct n as [|n]; simpl; case_nat n).
 
 Definition normally {R:Type} (f:steppable R) (P:R->Prop) : Prop :=
   forall s' n v rem,
@@ -60,27 +62,50 @@ Proof.
   case_nat n; crush.
 Qed.
 
+Definition write_pair a x := match x with (v1, v2) => 
+  do _ <- write a v1;
+  write (S a) v2
+  end.
+  
+Definition read_pair a :=
+  do v1 <- read a;
+  do v2 <- read (S a);
+  mret (v1, v2).
+
 Definition write_two a b :=
-  do _ <- write 0 a;
-  do _ <- write 1 b;
+  do _ <- write_pair 0 (a, b);
   do _ <- write 2 1;
   mret tt.
 
 Definition read_two :=
-  do a <- read 0;
-  do b <- read 1;
+  do x <- read_pair 0;
+  match x with (a, b) =>
   do c <- read 2;
-  mret (if eq_nat_dec c 1 then Some (a, b) else None).
+  mret (if eq_nat_dec c 1 then Some (a, b) else None)
+  end.
+
+Ltac flip_equality H :=
+  match goal with [ H : ?X = ?Y |- _ ] => let H1 := fresh "H" in rename H into H1; assert (H : Y = X) by (rewrite H1; reflexivity); clear H1 end.
+  
+Ltac clear_equalities :=
+  repeat match goal with
+  | [ |- ?X = ?Y -> _ ] => intro
+  | [ H : (_, _) = (_, _) |- _ ] => injection H; clear H
+  end.
+
+Ltac use_equalities :=
+  repeat match goal with
+  | [ H : ?X = ?Y |- _ ] => try rewrite H in *
+  end.
 
 Theorem pair_ok :
   forall a b,
   forall s n r s' n' r' res,
-  run (write_two a b) empty_storage n = (s, r) ->
-  run read_two s n' = (s', Some (res, r')) ->
+  (s, r) = run (write_two a b) empty_storage n ->
+  (s', Some (res, r')) = run read_two s n' ->
   res = None \/ res = Some (a, b).
 Proof.
-  intros a b s n r s' n' r' res.
-  unfold run, read_two, write_two.
+  intros a b s n r s' n' r' res. 
   simpl.
-  case_nat n; case_nat n'; try congruence; crush.
+  case_nat n; case_nat n'; try congruence; clear_equalities; use_equalities; crush.
 Qed.
